Add an initial disk to cache
Need to be able to roll back to old disk on miss

This should be wrapped up in the translator, so that from the outside
only cache_rep and a single disk are needed.

src/OptimisticCache.v
@@ -11,9 +11,13 @@ Require SepAuto.
 
 Definition Disk := @mem addr addr_eq_dec valu.
 
+Record CacheSt :=
+  caches { old_cache: Cache;
+           cache: Cache; }.
+
 Section OptimisticCache.
 
-  Implicit Types (c:Cache).
+  Implicit Types (c:Cache) (cs:CacheSt).
 
   Definition cache_rep (d: DISK) c (vd0: Disk) :=
     forall a, match cache_get c a with
@@ -32,17 +36,41 @@ Section OptimisticCache.
   with locking *)
   Variable G:Protocol.
 
-  Definition CacheRep d c (vd:Disk) :=
-    cache_rep d c vd.
+  Definition caches_consistent c0 c :=
+    (forall a, match cache_get c a with
+         | Present _ _ => True
+         | Invalid => cache_get c0 a = Invalid
+         | Missing => cache_get c0 a = Missing
+          end) /\
+    (forall a, match cache_get c0 a with
+          | Invalid => cache_get c a = Invalid
+          | _ => True
+          end).
 
-  Lemma CacheRep_fold : forall d c vd,
+  Definition CacheRep d cs (vd0 vd:Disk) :=
+    cache_rep d (old_cache cs) vd0 /\
+    cache_rep d (cache cs) vd /\
+    caches_consistent (old_cache cs) (cache cs).
+
+  Lemma CacheRep_fold : forall d c0 c vd0 vd,
+      cache_rep d c0 vd0 ->
       cache_rep d c vd ->
-      CacheRep d c vd.
+      caches_consistent c0 c ->
+      CacheRep d (caches c0 c) vd0 vd.
   Proof.
-    auto.
+    unfold CacheRep; intuition.
   Qed.
 
-  Hint Resolve CacheRep_fold.
+  Lemma CacheRep_fold' : forall d cs vd0 vd,
+      cache_rep d (old_cache cs) vd0 ->
+      cache_rep d (cache cs) vd ->
+      caches_consistent (old_cache cs) (cache cs) ->
+      CacheRep d cs vd0 vd.
+  Proof.
+    unfold CacheRep; intuition.
+  Qed.
+
+  Hint Resolve CacheRep_fold CacheRep_fold'.
 
   Ltac simplify :=
     repeat match goal with
@@ -50,7 +78,7 @@ Section OptimisticCache.
              let n := fresh n in
              let m := fresh m in
              destruct a as [m n]
-           | [ H: CacheRep _ _ _ |- _ ] =>
+           | [ H: CacheRep _ _ _ _ |- _ ] =>
              unfold CacheRep in H
            | [ |- exists (_: _ * _), _ ] => apply exists_tuple
            | [ H: (_, _) = (_, _) |- _ ] =>
@@ -76,38 +104,57 @@ Section OptimisticCache.
 
   Ltac step := CCLAutomation.step; simplify; finisher.
 
-  Definition ClearPending c a :=
+  Definition ClearPending cs a :=
     v <- WaitForRead a;
-      let c' := add_entry Clean c a v in
-        Ret (v, c').
+      let c0' := add_entry Clean (old_cache cs) a v in
+      let c' := add_entry Clean (cache cs) a v in
+        Ret (v, caches c0' c').
 
-  Definition CacheRead c a l :=
-    match cache_get c a with
-    | Present v _ => Ret (Some v, c)
+  Definition StartFill cs a :=
+    _ <- BeginRead a;
+      let c0' := mark_pending (old_cache cs) a in
+      let c' := mark_pending (cache cs) a in
+      Ret (caches c0' c').
+
+  Definition CacheRead cs a l :=
+    match cache_get (cache cs) a with
+    | Present v _ => Ret (Some v, cs)
     | Missing => if CanWrite l then
-                  _ <- BeginRead a;
-                  let c' := mark_pending c a in
-                  Ret (None, c')
-                else Ret (None, c)
+                  cs <- StartFill cs a;
+                    Ret (None, cs)
+                else Ret (None, cs)
     | Invalid => if CanWrite l then
-                  do '(v,c) <- ClearPending c a;
-                    Ret (Some v, c)
-                else Ret (None, c)
+                  do '(v,cs) <- ClearPending cs a;
+                    Ret (Some v, cs)
+                else Ret (None, cs)
+    end.
+
+  Ltac addrs_cases :=
+        match goal with
+        | [ a: addr, a': addr |- _ ] =>
+          destruct (addr_eq_dec a a'); subst;
+          autorewrite with cache upd in *;
+          try congruence
+        end.
+
+  Ltac specific_addr :=
+    match goal with
+    | [ a: addr, H: forall (_:addr), _ |- _ ] =>
+      lazymatch goal with
+      | [ a: addr, a': addr |- _ ] => fail
+      | _ => specialize (H a)
+      end
     end.
 
   Ltac solve_cache :=
     intuition;
-    try match goal with
+    repeat match goal with
         | [ H: cache_rep _ _ _ |- cache_rep _ _ _ ] =>
           unfold cache_rep in *;
           let a' := fresh "a'" in
           intro a';
           specialize (H a');
-          match goal with
-          | [ a: addr, a': addr |- _ ] =>
-            destruct (addr_eq_dec a a'); subst;
-            autorewrite with cache upd
-          end
+          addrs_cases
         | [ a: addr, H: cache_rep _ _ _ |- _ ] =>
           specialize (H a)
         end;
@@ -141,39 +188,76 @@ Section OptimisticCache.
 
   Hint Resolve cache_rep_finish_read.
 
-  Theorem ClearPending_ok : forall tid c a,
+  Lemma caches_consistent_c0_invalid : forall c0 c a,
+      caches_consistent c0 c ->
+      cache_get c a = Invalid ->
+      cache_get c0 a = Invalid.
+  Proof.
+    unfold caches_consistent; intuition.
+    specialize (H1 a); simpl_match; auto.
+  Qed.
+
+  Hint Resolve caches_consistent_c0_invalid.
+
+  Lemma cache_rep_invalid_same_val:
+    forall (a : addr) (vd0 vd : Disk) (v0 : valu) (st0 : Sigma)
+      (d : DISK) (c0 c : Cache),
+      cache_get c a = Invalid ->
+      caches_consistent c0 c ->
+      cache_rep d c0 vd0 ->
+      cache_rep d c vd ->
+      vd a = Some v0 ->
+      Sigma.disk st0 = upd d a (v0, NoReader) ->
+      vd0 a = Some v0.
+  Proof.
+    unfold caches_consistent; solve_cache.
+    repeat (specific_addr || simpl_match || deex).
+    congruence.
+  Qed.
+
+  Hint Resolve cache_rep_invalid_same_val.
+
+  Lemma caches_consistent_clean_entries:
+    forall (a : addr) (v0 : valu) (c0 c : Cache),
+      caches_consistent c0 c ->
+      caches_consistent (add_entry Clean c0 a v0) (add_entry Clean c a v0).
+  Proof.
+    unfold caches_consistent; intuition;
+      addrs_cases; eauto.
+    specialize (H0 a0).
+    destruct_all_matches.
+    specialize (H1 a0).
+    destruct_all_matches.
+  Qed.
+
+  Hint Resolve caches_consistent_clean_entries.
+
+  Theorem ClearPending_ok : forall tid cs a,
       cprog_spec G tid
-                 (fun '(F, vd, v0) sigma =>
+                 (fun '(F, vd0, vd, v0) sigma =>
                     {| precondition :=
                          F (Sigma.mem sigma) /\
-                         CacheRep (Sigma.disk sigma) c vd /\
-                         cache_get c a = Invalid /\
+                         CacheRep (Sigma.disk sigma) cs vd0 vd /\
+                         cache_get (cache cs) a = Invalid /\
                          vd a = Some v0 /\
                          Sigma.l sigma = WriteLock;
                        postcondition :=
-                         fun sigma' '(r, c') =>
+                         fun sigma' '(r, cs') =>
                            F (Sigma.mem sigma') /\
-                           CacheRep (Sigma.disk sigma') c' vd /\
-                           cache_get c' a = Present v0 Clean /\
+                           CacheRep (Sigma.disk sigma') cs' vd0 vd /\
+                           cache_get (cache cs') a = Present v0 Clean /\
                            r = v0 /\
                            Sigma.hm sigma' = Sigma.hm sigma /\
                            Sigma.l sigma' = Sigma.l sigma; |})
-                 (ClearPending c a).
+                 (ClearPending cs a).
   Proof.
     unfold ClearPending.
     hoare finish.
+    intuition finish.
+    eauto 10.
   Qed.
 
   Hint Extern 0 {{ ClearPending _ _; _ }} => apply ClearPending_ok : prog.
-
-  Lemma cache_rep_present_val:
-    forall (c : Cache) (a : addr) (v : valu) (b : DirtyBit),
-      cache_get c a = Present v b ->
-      forall (d : DISK) (vd : Disk) (v0 : valu),
-        cache_rep d c vd -> vd a = Some v0 -> v = v0.
-  Proof.
-    solve_cache.
-  Qed.
 
   Lemma cache_rep_missing_val:
     forall (c : Cache) (a : addr),
@@ -185,7 +269,7 @@ Section OptimisticCache.
     solve_cache.
   Qed.
 
-  Hint Resolve cache_rep_present_val cache_rep_missing_val.
+  Hint Resolve cache_rep_missing_val.
 
   Lemma cache_rep_start_fill:
     forall (c : Cache) (a : addr),
@@ -202,21 +286,102 @@ Section OptimisticCache.
 
   Hint Resolve cache_rep_start_fill.
 
-  Definition CacheRead_ok : forall tid c a l,
+  Lemma caches_consistent_c0_missing : forall c0 c a,
+      caches_consistent c0 c ->
+      cache_get c a = Missing ->
+      cache_get c0 a = Missing.
+  Proof.
+    unfold caches_consistent; intuition.
+    specialize (H1 a); simpl_match; auto.
+  Qed.
+
+  Hint Resolve caches_consistent_c0_missing.
+
+  Lemma cache_rep_missing_same_val:
+    forall (a : addr) (vd0 vd : Disk) (v0 : valu) (st0 : Sigma)
+      (d : DISK) (c0 c : Cache),
+      cache_get c a = Missing ->
+      caches_consistent c0 c ->
+      cache_rep d c0 vd0 ->
+      cache_rep d c vd ->
+      vd a = Some v0 ->
+      Sigma.disk st0 = upd d a (v0, Pending) ->
+      vd0 a = Some v0.
+  Proof.
+    unfold caches_consistent; solve_cache.
+    repeat (specific_addr || simpl_match || deex).
+    destruct (vd0 a); eauto.
+  Qed.
+
+  Hint Resolve cache_rep_missing_same_val.
+
+  Lemma cache_consistent_mark_pending:
+    forall (a : addr) (c0 c : Cache),
+      caches_consistent c0 c ->
+      caches_consistent (mark_pending c0 a) (mark_pending c a).
+  Proof.
+    unfold caches_consistent; intuition;
+      addrs_cases; eauto.
+    specialize (H0 a0).
+    destruct_all_matches.
+    specialize (H1 a0).
+    destruct_all_matches.
+  Qed.
+
+  Hint Resolve cache_consistent_mark_pending.
+
+  Theorem StartFill_ok : forall tid cs a,
       cprog_spec G tid
-                 (fun '(F, d, vd, v0) sigma =>
+                 (fun '(F, vd0, vd, v0) sigma =>
                     {| precondition :=
                          F (Sigma.mem sigma) /\
-                         CacheRep d c vd /\
+                         CacheRep (Sigma.disk sigma) cs vd0 vd /\
+                         cache_get (cache cs) a = Missing /\
+                         vd a = Some v0 /\
+                         Sigma.l sigma = WriteLock;
+                       postcondition :=
+                         fun sigma' cs' =>
+                           F (Sigma.mem sigma') /\
+                           CacheRep (Sigma.disk sigma') cs' vd0 vd /\
+                           cache_get (cache cs') a = Invalid /\
+                           Sigma.hm sigma' = Sigma.hm sigma /\
+                           Sigma.l sigma' = Sigma.l sigma; |})
+                 (StartFill cs a).
+  Proof.
+    unfold StartFill.
+    hoare finish.
+    intuition finish.
+    eauto 10.
+  Qed.
+
+  Hint Extern 1 {{ StartFill _ _; _ }} => apply StartFill_ok : prog.
+
+  Lemma cache_rep_present_val:
+    forall (c : Cache) (a : addr) (v : valu) (b : DirtyBit),
+      cache_get c a = Present v b ->
+      forall (d : DISK) (vd : Disk) (v0 : valu),
+        cache_rep d c vd -> vd a = Some v0 -> v = v0.
+  Proof.
+    solve_cache.
+  Qed.
+
+  Hint Resolve cache_rep_present_val.
+
+  Definition CacheRead_ok : forall tid cs a l,
+      cprog_spec G tid
+                 (fun '(F, d, vd0, vd, v0) sigma =>
+                    {| precondition :=
+                         F (Sigma.mem sigma) /\
+                         CacheRep d cs vd0 vd /\
                          (l = WriteLock -> d = Sigma.disk sigma) /\
                          Sigma.l sigma = l /\
                          vd a = Some v0;
                        postcondition :=
-                         fun sigma' '(r, c') =>
+                         fun sigma' '(r, cs') =>
                            F (Sigma.mem sigma') /\
                            let d' := if CanWrite l then Sigma.disk sigma' else d in
-                           CacheRep d' c' vd /\
-                           (l = Free -> c' = c) /\
+                           CacheRep d' cs' vd0 vd /\
+                           (l = Free -> cs' = cs) /\
                            (l = Free -> Sigma.disk sigma' = Sigma.disk sigma) /\
                            match r with
                            | Some v => v = v0
@@ -224,22 +389,22 @@ Section OptimisticCache.
                            end /\
                            Sigma.hm sigma' = Sigma.hm sigma /\
                            Sigma.l sigma' = Sigma.l sigma |})
-                 (CacheRead c a l).
+                 (CacheRead cs a l).
   Proof.
     unfold CacheRead.
     intros.
-    destruct (cache_get c a) eqn:?, (CanWrite l) eqn:?;
+    destruct (cache_get (cache cs) a) eqn:?, (CanWrite l) eqn:?;
              hoare finish.
   Qed.
 
-  Definition CacheWrite c a v :=
-    c <- match cache_get c a with
-        | Invalid => do '(_, c) <- ClearPending c a;
-                      Ret c
-        | _ => Ret c
+  Definition CacheWrite cs a v :=
+    cs <- match cache_get (cache cs) a with
+        | Invalid => do '(_, cs) <- ClearPending cs a;
+                      Ret cs
+        | _ => Ret cs
         end;
-      let c' := add_entry Dirty c a v in
-      Ret (tt, c').
+      let c' := add_entry Dirty (cache cs) a v in
+      Ret (tt, caches (old_cache cs) c').
 
   Lemma cache_rep_dirty_write:
     forall (c : Cache) (a : addr) (v : valu),
@@ -258,25 +423,118 @@ Section OptimisticCache.
   Hint Resolve cache_rep_dirty_write.
   Hint Extern 2 (cache_get _ _ <> _) => congruence.
 
-  Theorem CacheWrite_ok : forall tid c a v,
+  Lemma cache_consistent_add_dirty:
+    forall (a : addr) (v : valu) (c0 c : Cache),
+      cache_get c a <> Invalid ->
+      caches_consistent c0 c ->
+      caches_consistent c0 (add_entry Dirty c a v).
+  Proof.
+    unfold caches_consistent; intuition;
+      addrs_cases; eauto.
+    specialize (H1 a0).
+    destruct_all_matches; eauto.
+    specialize (H2 a0).
+    destruct_all_matches; try congruence; eauto.
+    specialize (H2 a0).
+    destruct_all_matches; try congruence; eauto.
+  Qed.
+
+  Hint Resolve cache_consistent_add_dirty.
+
+  Theorem CacheWrite_ok : forall tid cs a v,
       cprog_spec G tid
-                 (fun '(F, vd, v0) sigma =>
+                 (fun '(F, vd0, vd, v0) sigma =>
                     {| precondition :=
                          F (Sigma.mem sigma) /\
-                         CacheRep (Sigma.disk sigma) c vd /\
+                         CacheRep (Sigma.disk sigma) cs vd0 vd /\
                          vd a = Some v0 /\
                          Sigma.l sigma = WriteLock;
                        postcondition :=
-                         fun sigma' '(_, c') =>
+                         fun sigma' '(_, cs') =>
                            F (Sigma.mem sigma') /\
-                           CacheRep (Sigma.disk sigma') c' (upd vd a v) /\
+                           CacheRep (Sigma.disk sigma') cs' vd0 (upd vd a v) /\
                            Sigma.hm sigma' = Sigma.hm sigma /\
                            Sigma.l sigma' = Sigma.l sigma; |})
-                 (CacheWrite c a v).
+                 (CacheWrite cs a v).
   Proof.
     unfold CacheWrite.
     intros.
-    destruct (cache_get c a) eqn:?; hoare finish; simplify.
+    destruct (cache_get (cache cs) a) eqn:?; hoare finish.
+  Qed.
+
+  Definition CacheCommit cs :=
+    Ret (cache cs).
+
+  Theorem CacheCommit_ok : forall tid cs,
+      cprog_spec G tid
+                 (fun '(F, d, vd0, vd) sigma =>
+                    {| precondition :=
+                         F (Sigma.mem sigma) /\
+                         CacheRep d cs vd0 vd;
+                       postcondition :=
+                         fun sigma' c =>
+                           F (Sigma.mem sigma') /\
+                           cache_rep d c vd /\
+                           Sigma.disk sigma' = Sigma.disk sigma /\
+                           Sigma.hm sigma' = Sigma.hm sigma /\
+                           Sigma.l sigma' = Sigma.l sigma; |})
+                 (CacheCommit cs).
+  Proof.
+    unfold CacheCommit.
+    hoare finish.
+  Qed.
+
+  Definition CacheAbort cs :=
+    Ret (old_cache cs).
+
+  Theorem CacheAbort_ok : forall tid cs,
+      cprog_spec G tid
+                 (fun '(F, d, vd0, vd) sigma =>
+                    {| precondition :=
+                         F (Sigma.mem sigma) /\
+                         CacheRep d cs vd0 vd;
+                       postcondition :=
+                         fun sigma' c =>
+                           F (Sigma.mem sigma') /\
+                           cache_rep d c vd0 /\
+                           Sigma.disk sigma' = Sigma.disk sigma /\
+                           Sigma.hm sigma' = Sigma.hm sigma /\
+                           Sigma.l sigma' = Sigma.l sigma; |})
+                 (CacheAbort cs).
+  Proof.
+    unfold CacheAbort.
+    hoare finish.
+  Qed.
+
+  Definition CacheInit c :=
+    Ret (caches c c).
+
+  Lemma caches_consistent_refl : forall c,
+      caches_consistent c c.
+  Proof.
+    unfold caches_consistent; intuition;
+      destruct_all_matches.
+  Qed.
+
+  Hint Resolve caches_consistent_refl.
+
+  Theorem CacheInit_ok : forall tid c,
+      cprog_spec G tid
+                 (fun '(F, d, vd) sigma =>
+                    {| precondition :=
+                         F (Sigma.mem sigma) /\
+                         cache_rep d c vd;
+                       postcondition :=
+                         fun sigma' cs =>
+                           F (Sigma.mem sigma') /\
+                           CacheRep d cs vd vd /\
+                           Sigma.disk sigma' = Sigma.disk sigma /\
+                           Sigma.hm sigma' = Sigma.hm sigma /\
+                           Sigma.l sigma' = Sigma.l sigma; |})
+                 (CacheInit c).
+  Proof.
+    unfold CacheInit.
+    hoare finish.
   Qed.
 
 End OptimisticCache.
